refactored q7 to be alot cleaner

Assignment1/Ex7.dfy
@@ -32,50 +32,45 @@
 
 method Just1(a: array<int>, key: int) returns (b: bool)
 requires a != null
-ensures b ==> !VerifyCleanArray(a, key)
-ensures b ==> !VerifyArrayMoreThanOne(a, key)
-ensures forall i :: 0 <= i < a.Length ==> a[i] == old(a[i])
+ensures b == (CountOccurences(a, key, a.Length - 1) == 1)
+ensures forall i :: 0 <= i < a.Length ==> (a[i] == old(a[i]))
 {
-    b := false;
+
     var i := 0;
+    var count := 0;
     while i < a.Length
     invariant 0 <= i <= a.Length
-    invariant b ==> !forall j :: 0 <= j < i ==> (a[j] != key)
-    invariant b ==> forall j, k :: 0 <= j <= k < i && (a[j] == a[k]) && (a[j] == key) ==> (j == k)               
+    invariant count == CountOccurences(a, key, i-1)
     {
         if(a[i] == key)
         {
-            b := true;
-            var x := 0;
-            while x < a.Length
-            invariant 0 <= x <= a.Length
-            invariant b ==> forall j :: 0 <= j < x && (a[j] == key) ==> (j == i)
-            {
-                if(a[x] == key && x != i)
-                {
-                    b := false;
-                }
-
-                x := x + 1;
-            }
-            return;
+            count := count + 1;
         }
         i := i + 1;
     }
+    b := (count == 1);
 }
 
-predicate VerifyArrayMoreThanOne(a: array<int>, key: int)
-requires a != null;
-reads a;
+function CountOccurences(a: array<int>, key: int, index: int): int
+requires a != null
+requires index < a.Length
+// short circuit checking first :), this is only really here just so 
+// i can perform my assertions on occurences in array, no functional reason
+ensures (index >= 0 && a[index] == key) ==> (CountOccurences(a, key, index) == 1 + CountOccurences(a, key, index - 1))
+ensures (index >= 0 && a[index] != key) ==> (CountOccurences(a, key, index) ==  CountOccurences(a, key, index - 1))
+reads a
+// here i supply my variant that maxIndex is decreasing
+decreases index
 {
-    !(forall i, j :: 0 <= i <= j < a.Length && (a[i] == a[j]) && (a[i] == key) ==> (i == j))
-}
-
-predicate VerifyCleanArray(a: array<int>, key: int)
-requires a != null;
-reads a;
-{
-    forall i :: 0 <= i < a.Length ==> (a[i] != key)
+    if index < 0 
+    then
+        0
+    else
+        if a[index] == key 
+        then
+            CountOccurences(a, key, index - 1) + 1
+        else
+            CountOccurences(a, key, index - 1) 
 }
 
 predicate VerifyJustOne(a: array<int>, key: int)
@@ -100,8 +95,7 @@ method Main()
     assert testArray1[2] == 2;
     assert testArray1[3] == 1;
     var test1 := Just1(testArray1, 1);
-    assert !VerifyCleanArray(testArray1, 1);
-    assert VerifyArrayMoreThanOne(testArray1, 1);
+    assert (CountOccurences(testArray1, 1, testArray1.Length - 1) == 3);
     assert !VerifyJustOne(testArray1, 1);
     assert !test1;
 
@@ -111,10 +105,9 @@ method Main()
     assert testArray1[2] == 2;
     assert testArray1[3] == 1;
     var test2 := Just1(testArray1, 2);
-    assert !VerifyCleanArray(testArray1, 2);
-    assert !VerifyArrayMoreThanOne(testArray1, 2);
+    assert (CountOccurences(testArray1, 2, testArray1.Length - 1) == 1);
     assert VerifyJustOne(testArray1, 2);
-    assert test2 ==> !VerifyArrayMoreThanOne(testArray1, 2) && !VerifyCleanArray(testArray1, 2);
+    assert test2;
     
     assert testArray1.Length == 4;
     assert testArray1[0] == 1;
@@ -122,24 +115,29 @@ method Main()
     assert testArray1[2] == 2;
     assert testArray1[3] == 1;
     var test3 := Just1(testArray1, 3);
-    // // assert !VerifyJustOne(testArray1, 3);
-    // // assert test3 <==> (CountOccurencesFromZeroToIndex(testArray1, 3, testArray1.Length - 1) == 1);
+    assert (CountOccurences(testArray1, 3, testArray1.Length - 1) == 0);
+    assert !VerifyJustOne(testArray1, 3);
+    assert !test3;
 
     assert testArray2.Length == 1;
     assert testArray2[0] == 1;
     var test4 := Just1(testArray2, 1);
-    // // assert VerifyJustOne(testArray2, 1);
-    // // assert test4 <==> (CountOccurencesFromZeroToIndex(testArray2, 1, testArray2.Length - 1) == 1);
+    assert (CountOccurences(testArray2, 1, testArray2.Length - 1) == 1);
+    assert VerifyJustOne(testArray2, 1);
+    assert test4;
 
     assert testArray2.Length == 1;
     assert testArray2[0] == 1;
     var test5 := Just1(testArray2, 2);
-    // // assert !VerifyJustOne(testArray2, 2);
-    // // assert test5 <==> (CountOccurencesFromZeroToIndex(testArray2, 2, testArray2.Length - 1) == 1);
+    assert (CountOccurences(testArray2, 2, testArray2.Length - 1) == 0);
+    assert !VerifyJustOne(testArray2, 2);
+    assert !test5;
 
     assert testArray3.Length == 0;
     var test6 := Just1(testArray3, 1);
-    // // assert !VerifyJustOne(testArray3, 1);
+    assert (CountOccurences(testArray3, 1, testArray3.Length - 1) == 0);
+    assert !VerifyJustOne(testArray3, 1);
+    assert !test6;
 
     print test1, "\n", test2, "\n", test3, "\n", test4, "\n", test5, "\n", test6, "\n";
 }
